src/library/tactic/dsimplify.h
@@ -21,8 +21,9 @@ structure dsimp_config :=
 (eta : bool                := ff)
 (zeta : bool               := ff)
 (beta : bool               := tt)
-(proj : bool               := tt) -- reduce projections
+(proj : bool               := tt)
 (iota : bool               := tt)
+(unfold_reducible          := ff)
 (memoize                   := tt)
 */
 struct dsimp_config {
@@ -36,6 +37,7 @@ struct dsimp_config {
     bool                      m_beta;
     bool                      m_proj;
     bool                      m_iota;
+    bool                      m_unfold_reducible;
     bool                      m_memoize;
     dsimp_config();
     dsimp_config(vm_obj const & o);
@@ -69,15 +71,17 @@ public:
 
 class dsimplify_fn : public dsimplify_core_fn {
     simp_lemmas_for   m_simp_lemmas;
+    name_set          m_to_unfold;
     expr reduce(expr const & e);
     virtual optional<pair<expr, bool>> pre(expr const & e) override;
     virtual optional<pair<expr, bool>> post(expr const & e) override;
 public:
     dsimplify_fn(type_context & ctx, defeq_canonizer::state & s,
-                 simp_lemmas_for const & lemmas, dsimp_config const & cfg);
+                 simp_lemmas_for const & lemmas, list<name> const & to_unfold, dsimp_config const & cfg);
 };
 
 expr reduce_beta_eta_proj_iota(type_context & ctx, expr e, bool beta, bool eta, bool proj, bool iota);
+optional<expr> unfold_step(type_context & ctx, expr const & e, name_set const & to_unfold, bool unfold_reducible);
 
 void initialize_dsimplify();
 void finalize_dsimplify();
