tests/lean/dsimp_whnf.lean
@@ -2,6 +2,6 @@ open tactic
 
 example (a b : nat) : ((a + 1, b).1) = a + 1 :=
 by do
-  dsimp,
+  dsimp_target,
   trace_state,
   reflexivity
